better proofs

treiber_stack.v
@@ -5,12 +5,12 @@ From iris.heap_lang Require Import proofmode notation.
 From iris.algebra Require Import upred upred_big_op.
 From iris.tests Require Import atomic.
 
-Definition new_stack: val := λ: <>, ref NONE.
+Definition new_stack: val := λ: <>, ref (ref NONE).
 
 Definition push: val :=
   rec: "push" "s" "x" :=
       let: "hd" := !"s" in
-      let: "s'" := SOME ("x", ref "hd") in
+      let: "s'" := ref SOME ("x", "hd") in
       if: CAS "s" "hd" "s'"
         then #()
         else "push" "s" "x".
@@ -18,7 +18,7 @@ Definition push: val :=
 Definition pop: val :=
   rec: "pop" "s" :=
       let: "hd" := !"s" in
-      match: "hd" with
+      match: !"hd" with
         SOME "pair" =>
         if: CAS "s" "hd" (Snd "pair")
           then SOME (Fst "pair")
@@ -29,42 +29,30 @@ Definition pop: val :=
 Section proof.
   Context `{!heapG Σ} (N: namespace) (R: val → iProp Σ) `{∀ v, TimelessP (R v)}.
 
-  Fixpoint is_stack (s: loc) (xs: list val) : iProp Σ :=
+  Fixpoint is_stack' (hd: loc) (xs: list val) : iProp Σ :=
     match xs with
-    | [] => (s ↦ NONEV)%I
-    | x :: xs => (∃ s': loc, s ↦ SOMEV (x, #s') ★ R x ★ is_stack s' xs)%I
+    | [] => (∃ q, hd ↦{ q } NONEV)%I
+    | x :: xs => (∃ (hd': loc) q, hd ↦{ q } SOMEV (x, #hd') ★ □ R x ★ is_stack' hd' xs)%I
     end.
 
-  Definition is_some_stack (s: loc) : iProp Σ := (∃ xs: list val, is_stack s xs)%I.
+  Definition is_stack (s: loc) xs: iProp Σ := (∃ hd: loc, s ↦ #hd ★ is_stack' hd xs)%I.
 
-  Definition stack_inv s : iProp Σ := inv N (is_some_stack s).
-
-  Instance stack_inv_persistent s: PersistentP (stack_inv s).
-  Proof. apply _. Qed.
-
-  Instance is_stack_timeless: ∀ xs s, TimelessP (is_stack s xs).
-  Proof.
-    induction xs as [|? xs'].
-    - apply _.
-    - simpl. intros s.
-      apply uPred.exist_timeless.
-      intros s'. specialize IHxs' with s'.
-      apply _.
-  Qed.
-
-  Instance is_some_stack_timeless: ∀ s, TimelessP (is_some_stack s).
-  Proof.
-    intros s. rewrite /is_some_stack. apply uPred.exist_timeless. intros ?. apply is_stack_timeless.
-  Qed.
+  Definition is_some_stack (s: loc): iProp Σ := (∃ xs, is_stack s xs)%I.
 
   Lemma new_stack_spec:
     ∀ (Φ: val → iProp Σ),
       heapN ⊥ N →
       heap_ctx ★ (∀ s, is_stack s [] -★ Φ #s) ⊢ WP new_stack #() {{ Φ }}.
-  Proof. iIntros (Φ HN) "[#Hh HΦ]". wp_seq. wp_alloc l as "Hl". by iApply "HΦ". Qed.
+  Proof.
+    iIntros (Φ HN) "[#Hh HΦ]". wp_seq.
+    wp_bind (ref NONE)%E. wp_alloc l as "Hl".
+    wp_alloc l' as "Hl'".
+    iApply "HΦ". rewrite /is_stack. iExists l.
+    iFrame. by iExists 1%Qp.
+  Qed.
 
   Definition push_triple (s: loc) (x: val) :=
-    atomic_triple (fun xs => R x ★ is_stack s xs)%I
+    atomic_triple (fun xs => □ R x ★ is_stack s xs)%I
                   (fun xs _ => is_stack s (x :: xs))
                   (nclose heapN)
                   ⊤
@@ -73,56 +61,71 @@ Section proof.
   Lemma push_atomic_spec (s: loc) (x: val) :
     heapN ⊥ N → heap_ctx ⊢ push_triple s x.
   Proof.
-    iIntros (HN) "#?".
-    rewrite /push_triple /atomic_triple.
+    iIntros (HN) "#?". rewrite /push_triple /atomic_triple.
     iIntros (P Q) "#Hvs".
     iLöb as "IH". iIntros "!# HP". wp_rec.
     wp_let. wp_bind (! _)%E.
     iVs ("Hvs" with "HP") as (xs) "[[Hx Hxs] [Hvs' _]]".
-    destruct xs as [|y xs'].
-    - simpl. wp_load. iVs ("Hvs'" with "[Hx Hxs]") as "HP"; first by iFrame.
-      iVsIntro. wp_let. wp_alloc l as "Hl". wp_let.
-      wp_bind (CAS _ _ _)%E.
-      iVs ("Hvs" with "HP") as (xs) "[[Hx Hxs] Hvs']".
-      destruct xs as [|y xs'].
-      + simpl. wp_cas_suc.
-        iDestruct "Hvs'" as "[_ Hvs']".
-        iVs ("Hvs'" $! #() with "[Hl Hx Hxs]") as "HQ".
-        {  iExists l. by iFrame. }
-        iVsIntro. wp_if. iVsIntro. eauto.
-      + simpl. iDestruct "Hxs" as (s') "(Hs & Hy & Hs')".
-        wp_cas_fail.
-        iDestruct "Hvs'" as "[Hvs' _]".
-        iVs ("Hvs'" with "[Hx Hs Hy Hs']").
-        { iFrame. iExists s'. by iFrame. }
-        iVsIntro. wp_if. by iApply "IH".
-    - simpl.
-      iDestruct "Hxs" as (s') "(Hs & Hy & Hs')".
-      wp_load. iVs ("Hvs'" with "[Hx Hs Hy Hs']") as "HP".
-      { iFrame. iExists s'. by iFrame. }
-      iVsIntro. wp_let. wp_alloc l as "Hl".
-      wp_let. wp_bind (CAS _ _ _)%E.
-      iVs ("Hvs" with "HP") as (xs) "[[Hx Hxs] Hvs']".
-      destruct xs as [|y' xs''].
-      + simpl. wp_cas_fail.
-        iDestruct "Hvs'" as "[Hvs' _]".
-        iVs ("Hvs'" with "[Hx Hxs]"); first by iFrame.
-        iVsIntro. wp_if. by iApply "IH".
-      + simpl. iDestruct "Hxs" as (s'') "(Hs & Hy' & Hs'')".
-        destruct (decide (s' = s'' ∧ y = y')) as [[]|Hneq].
-        * subst. wp_cas_suc.
-          iDestruct "Hvs'" as "[_ Hvs']".
-          iVs ("Hvs'" $! #() with "[Hs Hx Hl Hy' Hs'']") as "HQ".
-          { iExists l. iFrame. iExists s''. by iFrame. }
-          iVsIntro. wp_if. iVsIntro. eauto.
-        * wp_cas_fail.
-          { intros Heq. apply Hneq. by inversion Heq. }
-          iDestruct "Hvs'" as "[Hvs' _]".
-          iVs ("Hvs'" with "[Hx Hs Hy' Hs'']").
-          { iFrame. iExists s''. by iFrame. }
-          iVsIntro. wp_if. by iApply "IH".
+    simpl. iDestruct "Hxs" as (hd) "[Hs Hhd]".
+    wp_load. iVs ("Hvs'" with "[Hx Hs Hhd]") as "HP".
+    { rewrite /is_stack. iFrame. iExists hd. by iFrame. }
+    iVsIntro. wp_let. wp_alloc l as "Hl". wp_let.
+    wp_bind (CAS _ _ _)%E.
+    iVs ("Hvs" with "HP") as (xs') "[[Hx Hxs] Hvs']".
+    simpl. iDestruct "Hxs" as (hd') "[Hs Hhd']".
+    destruct (decide (hd = hd')) as [->|Hneq].
+    * wp_cas_suc. iDestruct "Hvs'" as "[_ Hvs']".
+      iVs ("Hvs'" $! #() with "[-]") as "HQ".
+      {  iExists l. iFrame. iExists hd', 1%Qp. by iFrame. }
+      iVsIntro. wp_if. iVsIntro. eauto.
+    * wp_cas_fail.
+      iDestruct "Hvs'" as "[Hvs' _]".
+      iVs ("Hvs'" with "[-]") as "HP".
+      {  iFrame. iExists hd'. by iFrame. }
+      iVsIntro. wp_if. by iApply "IH".
   Qed.
+
+  Definition pop_triple (s: loc) :=
+    atomic_triple (fun xs => is_stack s xs)%I
+                  (fun xs ret => ret = NONEV ∨ (∃ x, ret = SOMEV x ★ □ R x))%I (* FIXME: we can give a stronger one *)
+                  (nclose heapN)
+                  ⊤
+                  (pop #s).
   
-    
+  Lemma pop_atomic_spec (s: loc) (x: val) :
+    heapN ⊥ N → heap_ctx ⊢ pop_triple s.
+  Proof.
+    iIntros (HN) "#?".
+    rewrite /pop_triple /atomic_triple.
+    iIntros (P Q) "#Hvs".
+    iLöb as "IH". iIntros "!# HP". wp_rec.
+    wp_bind (! _)%E.
+    iVs ("Hvs" with "HP") as (xs) "[Hxs Hvs']".
+    destruct xs as [|y' xs'].
+    - simpl. iDestruct "Hxs" as (hd) "[Hs Hhd]".
+      wp_load. iDestruct "Hvs'" as "[_ Hvs']".
+      iVs ("Hvs'" $! NONEV with "[]") as "HQ"; first by iLeft.
+      iVsIntro. wp_let. iDestruct "Hhd" as (q) "Hhd".
+      wp_load. wp_match.
+      iVsIntro. by iExists [].
+    - simpl. iDestruct "Hxs" as (hd) "[Hs Hhd]".
+      simpl. iDestruct "Hhd" as (hd' q) "([Hhd Hhd'] & #Hy' & Hxs')".
+      wp_load. iDestruct "Hvs'" as "[Hvs' _]".
+      iVs ("Hvs'" with "[-Hhd]") as "HP".
+      { iExists hd. iFrame. iExists hd', (q / 2)%Qp. by iFrame. }
+      iVsIntro. wp_let. wp_load. wp_match. wp_proj.
+      wp_bind (CAS _ _ _). iVs ("Hvs" with "HP") as (xs) "[Hxs Hvs']".
+      iDestruct "Hxs" as (hd'') "[Hs Hhd'']".
+      destruct (decide (hd = hd'')) as [->|Hneq].
+      + wp_cas_suc. iDestruct "Hvs'" as "[_ Hvs']".
+        iVs ("Hvs'" $! (SOMEV y') with "[]") as "HQ".
+        { iRight. eauto. }
+        iVsIntro. wp_if. wp_proj. eauto.
+      + wp_cas_fail. iDestruct "Hvs'" as "[Hvs' _]".
+        iVs ("Hvs'" with "[-]") as "HP".
+        { iExists hd''. by iFrame. }
+        iVsIntro. wp_if. by iApply "IH".
+  Qed.
+      
 End proof.
 
